OpenvmFv.lean
@@ -103,6 +103,7 @@ import OpenvmFv.Spec.ITYPE.xori
 import OpenvmFv.Spec.ITYPE.slti
 import OpenvmFv.Spec.ITYPE.sltiu
 import OpenvmFv.Spec.JAL.execute_jal
+import OpenvmFv.Spec.Load.local2
 import OpenvmFv.Spec.RTYPE.add
 import OpenvmFv.Spec.RTYPE.and
 import OpenvmFv.Spec.RTYPE.local
