OpenvmFv/Spec/Load/lw.lean
@@ -1,0 +1,379 @@
+import OpenvmFv.Spec.Load.local2
+import OpenvmFv.Spec.rX_bits
+
+namespace PureSpec
+
+  structure LwInput where
+    -- operands
+    r1 : BitVec 5
+    imm : BitVec 12
+    rd : BitVec 5
+    -- registers
+    r1_val : BitVec 32
+    PC : BitVec 32
+    mstatus : BitVec 64
+    cur_privilege : Privilege
+    plat_clint_base : BitVec 34
+    plat_clint_size : BitVec 34
+    plat_ram_base : BitVec 34
+    plat_ram_size : BitVec 34
+    plat_rom_base : BitVec 34
+    plat_rom_size : BitVec 34
+    htif_tohost_base : Option (BitVec 34)
+    -- memory
+    data0 : BitVec 8
+    data1 : BitVec 8
+    data2 : BitVec 8
+    data3 : BitVec 8
+
+  structure LwOutput where
+    -- registers
+    nextPC : BitVec 32
+    rd : Option (Finset.Icc 1 31 × BitVec 32)
+
+  def execute_LOAD_lw_pure (input : LwInput) : LwOutput := {
+    nextPC := input.PC + 4#32
+    rd := if h: input.rd = 0
+      then .none
+      else .some (
+        ⟨
+          input.rd.toNat,
+          by
+            apply Finset.mem_Icc.mpr;
+            done
+        ⟩,
+        input.data3 ++ input.data2 ++ input.data1 ++ input.data0
+      )
+    : LwOutput
+  }
+
+  def bitvec_to_reg (bv: BitVec 5) : Register :=
+    match bv with
+      | 0#5 => Register.x1 -- purely used for totality, does not come up
+      | 1#5 => Register.x1
+      | 2#5 => Register.x2
+      | 3#5 => Register.x3
+      | 4#5 => Register.x4
+      | 5#5 => Register.x5
+      | 6#5 => Register.x6
+      | 7#5 => Register.x7
+      | 8#5 => Register.x8
+      | 9#5 => Register.x9
+      | 10#5 => Register.x10
+      | 11#5 => Register.x11
+      | 12#5 => Register.x12
+      | 13#5 => Register.x13
+      | 14#5 => Register.x14
+      | 15#5 => Register.x15
+      | 16#5 => Register.x16
+      | 17#5 => Register.x17
+      | 18#5 => Register.x18
+      | 19#5 => Register.x19
+      | 20#5 => Register.x20
+      | 21#5 => Register.x21
+      | 22#5 => Register.x22
+      | 23#5 => Register.x23
+      | 24#5 => Register.x24
+      | 25#5 => Register.x25
+      | 26#5 => Register.x26
+      | 27#5 => Register.x27
+      | 28#5 => Register.x28
+      | 29#5 => Register.x29
+      | 30#5 => Register.x30
+      | 31#5 => Register.x31
+      | _ => Register.x1
+
+  def lw_state_assumptions
+    (i : LwInput)
+    (state : PreSail.SequentialState RegisterType Sail.trivialChoiceSource)
+  : Prop :=
+    LeanRV32D.Functions.is_aligned_vaddr (virtaddr.Virtaddr (i.r1_val + (BitVec.signExtend 32 i.imm))) 4 = true ∧
+    LeanRV32D.Functions.rX_bits (regidx.Regidx i.r1) state = EStateM.Result.ok i.r1_val state ∧
+    Sail.readReg Register.mstatus state = EStateM.Result.ok i.mstatus state ∧
+    Sail.readReg Register.cur_privilege state = EStateM.Result.ok i.cur_privilege state ∧
+    Sail.readReg Register.plat_clint_base state = EStateM.Result.ok i.plat_clint_base state ∧
+    Sail.readReg Register.plat_clint_size state = EStateM.Result.ok i.plat_clint_size state ∧
+    Sail.readReg Register.plat_ram_base state = EStateM.Result.ok i.plat_ram_base state ∧
+    Sail.readReg Register.plat_rom_base state = EStateM.Result.ok i.plat_rom_base state ∧
+    Sail.readReg Register.plat_ram_size state = EStateM.Result.ok i.plat_ram_size state ∧
+    Sail.readReg Register.plat_rom_size state = EStateM.Result.ok i.plat_rom_size state ∧
+    Sail.readReg Register.htif_tohost_base state = EStateM.Result.ok i.htif_tohost_base state ∧
+    state.mem[i.r1_val.toNat + (BitVec.signExtend 32 i.imm).toNat]? = .some i.data0 ∧
+    state.mem[i.r1_val.toNat + (BitVec.signExtend 32 i.imm).toNat + 1]? = .some i.data1 ∧
+    state.mem[i.r1_val.toNat + (BitVec.signExtend 32 i.imm).toNat + 2]? = .some i.data2 ∧
+    state.mem[i.r1_val.toNat + (BitVec.signExtend 32 i.imm).toNat + 3]? = .some i.data3 ∧
+    state.regs.get? Register.PC = .some i.PC ∧
+    i.cur_privilege = Privilege.Machine ∧
+    i.plat_clint_base = 0 ∧
+    i.plat_clint_size = 0 ∧
+    i.plat_ram_base = 0 ∧
+    i.plat_ram_size = (BitVec.ofNat 34 (2^32 - 1)) ∧
+    i.plat_rom_base = 0 ∧
+    i.htif_tohost_base = .none ∧
+    BitVec.extractLsb 17 17 i.mstatus = 0#1 ∧
+    i.r1_val.toNat + (BitVec.signExtend 32 i.imm).toNat + 4 < 2^32
+
+  set_option maxHeartbeats 0 in
+  lemma execute_LOAD_lw_pure_equiv
+    (lw_input : LwInput)
+    (h_assumptions : lw_state_assumptions lw_input state)
+  :
+    (
+      do
+        Sail.writeReg Register.nextPC (Sail.BitVec.addInt (← Sail.readReg Register.PC) 4)
+        LeanRV32D.Functions.execute (instruction.LOAD (
+          lw_input.imm,
+          regidx.Regidx lw_input.r1,
+          regidx.Regidx lw_input.rd,
+          true,
+          4
+        ))
+    ) state =
+    let lw_output := execute_LOAD_lw_pure lw_input
+    (do
+      Sail.writeReg Register.nextPC lw_output.nextPC
+      match lw_output.rd with
+        | .some (rd, rd_val) => write_xreg rd rd_val
+        | .none => pure ()
+      pure (ExecutionResult.Retire_Success ())
+    ) state
+  := by
+    obtain ⟨
+      h_aligned,
+      h_r1_val,
+      h_mstatus,
+      h_cur_privilege,
+      h_clint_base,
+      h_clint_size,
+      h_plat_ram_base,
+      h_plat_rom_base,
+      h_plat_ram_size,
+      h_plat_rom_size,
+      h_htif_tohost_base,
+      h_mem_0,
+      h_mem_1,
+      h_mem_2,
+      h_mem_3,
+      h_pc,
+      h_cur_privilege_val,
+      h_plat_clint_base_val,
+      h_plat_clint_size_val,
+      h_plat_ram_base_val,
+      h_plat_ram_size_val,
+      h_plat_rom_base_val,
+      h_htif_tohost_base_val,
+      h_mstatus_val,
+      h_does_fit
+    ⟩ := h_assumptions
+
+    rewrite [h_cur_privilege_val] at h_cur_privilege
+    rewrite [h_plat_clint_base_val] at h_clint_base
+    rewrite [h_plat_clint_size_val] at h_clint_size
+    rewrite [h_plat_ram_base_val] at h_plat_ram_base
+    rewrite [h_plat_ram_size_val] at h_plat_ram_size
+    rewrite [h_plat_rom_base_val] at h_plat_rom_base
+    rewrite [h_htif_tohost_base_val] at h_htif_tohost_base
+
+
+    simp [
+      readReg_state h_pc,
+      writeReg_state_success,
+    ]
+
+    rewrite [
+      Local.execute_load_instruction,
+      ←Local.execute_LOAD_equiv
+    ]
+    simp
+
+    set state' := (write_reg_state state Register.nextPC (Sail.BitVec.addInt lw_input.PC 4)) with h_state'
+
+    replace h_r1_val : LeanRV32D.Functions.rX_bits (regidx.Regidx lw_input.r1) state' = EStateM.Result.ok lw_input.r1_val state' := by
+      clear *- h_r1_val h_state'
+      rewrite [h_state']
+      by_cases h_r1: lw_input.r1 = 0
+      . simp [
+         h_r1, LeanRV32D.Functions.rX_bits, LeanRV32D.Functions.rX
+        ] at ⊢ h_r1_val
+        exact h_r1_val
+      by_cases h_r1 : lw_input.r1 = 1 <;> [
+        skip ; by_cases h_r1 : lw_input.r1 = 2 <;> [
+        skip ; by_cases h_r1 : lw_input.r1 = 3 <;> [
+        skip ; by_cases h_r1 : lw_input.r1 = 4 <;> [
+        skip ; by_cases h_r1 : lw_input.r1 = 5 <;> [
+        skip ; by_cases h_r1 : lw_input.r1 = 6 <;> [
+        skip ; by_cases h_r1 : lw_input.r1 = 7 <;> [
+        skip ; by_cases h_r1 : lw_input.r1 = 8 <;> [
+        skip ; by_cases h_r1 : lw_input.r1 = 9 <;> [
+        skip ; by_cases h_r1 : lw_input.r1 = 10 <;> [
+        skip ; by_cases h_r1 : lw_input.r1 = 11 <;> [
+        skip ; by_cases h_r1 : lw_input.r1 = 12 <;> [
+        skip ; by_cases h_r1 : lw_input.r1 = 13 <;> [
+        skip ; by_cases h_r1 : lw_input.r1 = 14 <;> [
+        skip ; by_cases h_r1 : lw_input.r1 = 15 <;> [
+        skip ; by_cases h_r1 : lw_input.r1 = 16 <;> [
+        skip ; by_cases h_r1 : lw_input.r1 = 17 <;> [
+        skip ; by_cases h_r1 : lw_input.r1 = 18 <;> [
+        skip ; by_cases h_r1 : lw_input.r1 = 19 <;> [
+        skip ; by_cases h_r1 : lw_input.r1 = 20 <;> [
+        skip ; by_cases h_r1 : lw_input.r1 = 21 <;> [
+        skip ; by_cases h_r1 : lw_input.r1 = 22 <;> [
+        skip ; by_cases h_r1 : lw_input.r1 = 23 <;> [
+        skip ; by_cases h_r1 : lw_input.r1 = 24 <;> [
+        skip ; by_cases h_r1 : lw_input.r1 = 25 <;> [
+        skip ; by_cases h_r1 : lw_input.r1 = 26 <;> [
+        skip ; by_cases h_r1 : lw_input.r1 = 27 <;> [
+        skip ; by_cases h_r1 : lw_input.r1 = 28 <;> [
+        skip ; by_cases h_r1 : lw_input.r1 = 29 <;> [
+        skip ; by_cases h_r1 : lw_input.r1 = 30 <;> [
+        skip ; by_cases h_r1 : lw_input.r1 = 31 <;> [
+          skip; (exfalso; grind)
+        ]
+      ]]]]]]]]]]]]]]]]]]]]]]]]]]]]]]
+      all_goals {
+        simp [
+          h_r1, LeanRV32D.Functions.rX_bits, LeanRV32D.Functions.rX,
+          Sail.readReg, PreSail.readReg, write_reg_state,
+          LeanRV32D.Functions.regval_from_reg
+        ] at ⊢ h_r1_val
+        unfold get instMonadStateOfMonadStateOf getThe MonadStateOf.get EStateM.instMonadStateOf EStateM.get at ⊢ h_r1_val
+        dsimp at ⊢ h_r1_val
+        have :
+          (state.regs.insert Register.nextPC (Sail.BitVec.addInt lw_input.PC 4)).get? (bitvec_to_reg lw_input.r1) =
+          state.regs.get? (bitvec_to_reg lw_input.r1)
+        := by rewrite [h_r1]; simp [bitvec_to_reg]; grind
+        rewrite [h_r1] at this
+        simp [bitvec_to_reg] at this
+        simp [this]
+        have : ∃ x_val, state.regs.get? (bitvec_to_reg lw_input.r1) = .some x_val := by
+          by_cases h_contr : ∃ x_val, state.regs.get? (bitvec_to_reg lw_input.r1) = .some x_val
+          . assumption
+          . rewrite [h_r1] at h_contr
+            simp [bitvec_to_reg] at h_contr
+            apply Option.eq_none_iff_forall_ne_some.mpr at h_contr
+            simp [h_contr] at h_r1_val
+            done
+        rewrite [h_r1] at this
+        simp [bitvec_to_reg] at this
+        obtain ⟨x, h_x⟩ := this
+        simp [h_x] at ⊢ h_r1_val
+        exact h_r1_val
+      }
+
+    replace h_mstatus :
+      Sail.readReg Register.mstatus state' =
+      EStateM.Result.ok lw_input.mstatus state'
+    := by
+      rewrite [h_state']
+      clear *-h_mstatus
+      simp [
+        Sail.readReg, PreSail.readReg, write_reg_state
+      ] at ⊢ h_mstatus
+      unfold get instMonadStateOfMonadStateOf getThe MonadStateOf.get EStateM.instMonadStateOf EStateM.get at ⊢ h_mstatus
+      dsimp at ⊢ h_mstatus
+      have :
+        (state.regs.insert Register.nextPC (Sail.BitVec.addInt lw_input.PC 4)).get? Register.mstatus =
+        state.regs.get? Register.mstatus
+      := by grind
+      simp [this, h_mstatus]
+      done
+
+
+
+
+    have h_execute_load := Local.execute_LOAD_simplified
+      state'
+      (regidx.Regidx lw_input.rd)
+      lw_input.data0
+      lw_input.data1
+      lw_input.data2
+      lw_input.data3
+      h_aligned
+      h_r1_val
+      -- h_mstatus
+      -- h_cur_privilege
+      -- h_clint_base
+      -- h_clint_size
+      -- h_plat_ram_base
+      -- h_plat_rom_base
+      -- h_plat_ram_size
+      -- h_plat_rom_size
+      -- h_htif_tohost_base
+      -- h_mstatus_val
+      -- h_does_fit
+      -- h_mem_0
+      -- h_mem_1
+      -- h_mem_2
+      -- h_mem_3
+
+    rewrite [
+      Local.execute_LOAD_equiv,
+      h_execute_load
+    ]
+
+
+
+    unfold bind Monad.toBind EStateM.instMonad
+    dsimp
+    unfold EStateM.bind
+    dsimp
+
+    simp [
+      readReg_state h_input_pc,
+      writeReg_state_success,
+      ←Local.execute_equiv,
+      Local.execute.eq_def
+    ]
+
+    have (x : BitVec 32) : Sail.BitVec.addInt x 4 = x + 4 := rfl
+    simp [this]
+
+    have := Local.execute_LOAD_simplified
+      lw_input.data0
+      lw_input.data1
+      lw_input.data2
+      lw_input.data3
+
+
+    simp [
+      Local.execute_LOAD_simplified
+    ]
+
+    simp [
+      ←Local.execute_RTYPE_equiv,
+      Local.execute_RTYPE.eq_def,
+      bind, EStateM.instMonad, EStateM.bind
+    ]
+
+    rewrite [rX_read_xreg_equiv _ r1 (regidx_to_fin r1) (by simp [regidx_to_fin])]
+    rewrite [read_xreg_write_reg_state_nextPC _ h_input_r1]
+    simp
+    rewrite [rX_read_xreg_equiv _ r2 (regidx_to_fin r2) (by simp [regidx_to_fin])]
+    rewrite [read_xreg_write_reg_state_nextPC _ h_input_r2]
+    simp [EStateM.pure]
+
+    simp [execute_RTYPE_add_pure]
+
+    obtain ⟨rd⟩ := rd
+    by_cases h_zero: rd = 0
+    . rewrite [h_zero, wX_write_xreg_0_equiv]
+      simp
+      rewrite [dite_cond_eq_true]
+      . simp
+      . simp [h_input_rd, h_zero, regidx_to_fin]
+    . have h_inc := regidx_non_zero h_zero
+      apply Finset.mem_Icc.mp at h_inc
+      obtain ⟨h_low, h_high⟩ := h_inc
+      rewrite [
+        wX_write_xreg_equiv _ _
+          (regidx.Regidx rd)
+          ⟨(regidx_to_fin (regidx.Regidx rd)).val, Finset.mem_Icc.mpr ⟨h_low, h_high⟩⟩
+          (by simp [regidx_to_fin])
+      ]
+      simp [regidx_to_fin]
+      rewrite [dite_cond_eq_false]
+      . simp [h_input_rd, regidx_to_fin]
+      . simp [regidx_to_fin] at *
+        omega
+
+end PureSpec
